ThoR/Semantics/Semantics.lean
@@ -6,8 +6,6 @@ Authors: s. file CONTRIBUTORS
 
 import ThoR.Relation.Rel
 
--- FIXME: Präzedenzen der Operatoren mit Lean.Notation abgleichen
-
 namespace ThoR.Semantics
 
 variable {R : Type} [TupleSet R]
@@ -26,14 +24,9 @@ mutual
     | append {n : ℕ} {t1 t2 : RelType R n} (r1 : Rel t1) (r2 : Rel t2) : Expression (t1 ++ t2)
     | domrestr {n : ℕ} {t1 : RelType R 1} {t2 : RelType R n} (r1 : Rel t1) (r2 : Rel t2) : Expression (t1 <: t2)
     | rangerestr {n : ℕ} {t1 : RelType R n} {t2 : RelType R 1} (r1 : Rel t1) (r2 : Rel t2) : Expression (t1 :> t2)
-    -- | if_then_else {n : ℕ} {t1 t2 : RelType R n} (f : Formula) (r1 : Rel t1) (r2 : Rel t2) : Expression ?
+    | if_then_else {n : ℕ} {t1 t2 : RelType R n} (f : Formula) (r1 : Rel t1) (r2 : Rel t2) : Expression (RelType.ifThenElse t1 t2)
 -- function
 -- let
-
-  inductive TypeExpression : ℕ → Type u where
-    | unary_rel {t : RelType R 1} (m : Shared.mult) (r : Rel t) : TypeExpression n
-    | rel {n : ℕ} {t : RelType R n} (r : Rel t) : TypeExpression n
-    | complex {n1 n2 : ℕ} (te1 : TypeExpression n1) (te2: TypeExpression n2) : TypeExpression (n1 + n2)
 
   inductive ArithmeticExpression : Type u where
     | number (z : ℤ) : ArithmeticExpression
@@ -64,23 +57,64 @@ mutual
     | in {n : ℕ} {t1 t2 : RelType R n} (e1 : Expression t1) (e2 : Expression t2): Formula
     | eq {n : ℕ} {t1 t2 : RelType R n} (e1 : Expression t1) (e2 : Expression t2) : Formula
     | neq {n : ℕ} {t1 t2 : RelType R n} (e1 : Expression t1) (e2 : Expression t2) : Formula
+-- pred
+
+  inductive TypeExpression : ℕ → Type u where
+    | type {n : ℕ} (t : RelType R n) : TypeExpression n
 end
 
 mutual
-  def Expression.eval {n : ℕ } {t : RelType R n} (e : Expression t) :=
+  def Expression.eval {n : ℕ } {t : RelType R n} (e : @Expression R _ _ t) :=
     match e with
-    | rel           r       => r
-    | intersect     r1 r2   => r1 & r2
-    | union         r1 r2   => r1 + r2
-    | diff          r1 r2   => r1 -r2
-    | cartprod      r1 r2   => r1 ⟶ r2
-    | dotjoin       r1 r2   => r1 ⋈ r2
-    | transclos     r       => ^ r
-    | reftransclos  r       => * r
-    | transpose     r       => ~ r
-    | append        r1 r2   => r1 ++ r2
-    | domrestr      r1 r2   => r1 <: r2
-    | rangerestr    r1 r2   => r1 :> r2
+    | .rel           r       => r
+    | .intersect     r1 r2   => r1 & r2
+    | .union         r1 r2   => r1 + r2
+    | .diff          r1 r2   => r1 -r2
+    | .cartprod      r1 r2   => r1 ⟶ r2
+    | .dotjoin       r1 r2   => r1 ⋈ r2
+    | .transclos     r       => ^ r
+    | .reftransclos  r       => * r
+    | .transpose     r       => ~ r
+    | .append        r1 r2   => r1 ++ r2
+    | .domrestr      r1 r2   => r1 <: r2
+    | .rangerestr    r1 r2   => r1 :> r2
+    | .if_then_else  f r1 r2 => HIfThenElse.hIfThenElse f.eval r1 r2
+
+  def ArithmeticExpression.eval (a : @ArithmeticExpression R _) :=
+    match a with
+    | .number   z     => z
+    | .negation a     => - a.eval
+    | .add      a1 a2 => a1.eval + a2.eval
+    | .sub      a1 a2 => a1.eval - a2.eval
+    | .mult     a1 a2 => a1.eval * a2.eval
+    | .div      a1 a2 => a1.eval / a2.eval
+    | .rem      a1 a2 => a1.eval % a2.eval
+    | .card     r     => Card.card r
+
+  def Formula.eval (f : @Formula R _) :=
+    match f with
+    | .no           e         => SetMultPredicates.no e.eval
+    | .lone         e         => SetMultPredicates.lone e.eval
+    | .one          e         => SetMultPredicates.one e.eval
+    | .some         e         => SetMultPredicates.some e.eval
+    | .not          f         => ¬ f.eval
+    | .or           f1 f2     => f1.eval ∨ f2.eval
+    | .and          f1 f2     => f1.eval ∧ f2.eval
+    | .equivalent   f1 f2     => f1.eval ↔ f2.eval
+    | .implication  f1 f2     => f1.eval → f2.eval
+    | .if_then_else f f1 f2   => (f.eval → f1.eval) ∧ (¬ f.eval → f2.eval)
+    | .a_lt         a1 a2     => a1.eval < a2.eval
+    | .a_gt         a1 a2     => a1.eval > a2.eval
+    | .a_eq         a1 a2     => a1.eval = a2.eval
+    | .a_leq        a1 a2     => a1.eval ≤ a2.eval
+    | .a_geq        a1 a2     => a1.eval ≥ a2.eval
+    | .in           r1 r2     => r1.eval ⊂ r2.eval
+    | .eq           r1 r2     => r1.eval ≡ r2.eval
+    | .neq          r1 r2     => ¬ (r1.eval ≡ r2.eval)
+
+  def TypeExpression.eval {n : ℕ} (te : @TypeExpression R _ n) :=
+    match te with
+    | .type t => t
 end
 
 end ThoR.Semantics
